PrimParser.lean
@@ -1,5 +1,6 @@
 import PrimParser.Base
 import PrimParser.Basic
+import PrimParser.Grade
 import PrimParser.GradedMonad
 import PrimParser.Necessity
 import PrimParser.Properties
